Foundation/Modal/Logic/WellKnown.lean
@@ -2,9 +2,18 @@ import Foundation.Modal.Hilbert.Maximal.Unprovability
 import Foundation.Modal.Kripke.Hilbert.GL.Completeness
 import Foundation.Modal.Kripke.Hilbert.Grz.Completeness
 import Foundation.Modal.Kripke.Hilbert.K4
+import Foundation.Modal.Kripke.Hilbert.K45
 import Foundation.Modal.Kripke.Hilbert.K5
+import Foundation.Modal.Kripke.Hilbert.KB
+import Foundation.Modal.Kripke.Hilbert.KB4
+import Foundation.Modal.Kripke.Hilbert.KB5
 import Foundation.Modal.Kripke.Hilbert.KD
+import Foundation.Modal.Kripke.Hilbert.KD4
+import Foundation.Modal.Kripke.Hilbert.KD45
+import Foundation.Modal.Kripke.Hilbert.KD5
+import Foundation.Modal.Kripke.Hilbert.KDB
 import Foundation.Modal.Kripke.Hilbert.KT
+import Foundation.Modal.Kripke.Hilbert.KTB
 import Foundation.Modal.Kripke.Hilbert.S4
 import Foundation.Modal.Kripke.Hilbert.S5
 import Foundation.Modal.Kripke.Hilbert.Triv
@@ -17,81 +26,97 @@ namespace LO.Modal
 namespace Logic
 
 protected abbrev K4 : Logic := Hilbert.K4.logic
-
-instance : (Logic.K4).Normal := Hilbert.normal
-
 lemma K4.eq_TransitiveKripkeFrameClass_Logic : Logic.K4 = Kripke.TransitiveFrameClass.logic
   := eq_Hilbert_Logic_KripkeFrameClass_Logic
 
 
-protected abbrev KD : Logic := Hilbert.KD.logic
-
-instance : (Logic.KD).Normal := Hilbert.normal
-
-lemma KD.eq_SerialKripkeFrameClass_Logic : Logic.KD = Kripke.SerialFrameClass.logic
-  := eq_Hilbert_Logic_KripkeFrameClass_Logic
-
-
-protected abbrev KT : Logic := Hilbert.KT.logic
-
-instance : (Logic.KT).Normal := Hilbert.normal
-
-lemma KT.eq_TransitiveKripkeFrameClass_Logic : Logic.KT = Kripke.ReflexiveFrameClass.logic
+protected abbrev K45 : Logic := Hilbert.K45.logic
+lemma K45.eq_TransitiveEuclideanKripkeFrameClass_Logic : Logic.K45 = Kripke.TransitiveEuclideanFrameClass.logic
   := eq_Hilbert_Logic_KripkeFrameClass_Logic
 
 
 protected abbrev K5 : Logic := Hilbert.K5.logic
-
-instance : (Logic.K5).Normal := Hilbert.normal
-
 lemma K5.eq_EuclideanKripkeFrameClass_Logic : Logic.K5 = Kripke.EuclideanFrameClass.logic
   := eq_Hilbert_Logic_KripkeFrameClass_Logic
 
 
+protected abbrev KB : Logic := Hilbert.KB.logic
+lemma KB.eq_SymmetricKripkeFrameClass_Logic : Logic.KB = Kripke.SymmetricFrameClass.logic
+  := eq_Hilbert_Logic_KripkeFrameClass_Logic
+
+
+protected abbrev KB4 : Logic := Hilbert.KB4.logic
+lemma KB4.eq_ReflexiveTransitiveKripkeFrameClass_Logic : Logic.KB4 = Kripke.SymmetricTransitiveFrameClass.logic
+  := eq_Hilbert_Logic_KripkeFrameClass_Logic
+
+
+protected abbrev KB5 : Logic := Hilbert.KB5.logic
+lemma KB5.eq_ReflexiveEuclideanKripkeFrameClass_Logic : Logic.KB5 = Kripke.SymmetricEuclideanFrameClass.logic
+  := eq_Hilbert_Logic_KripkeFrameClass_Logic
+
+
+protected abbrev KD : Logic := Hilbert.KD.logic
+lemma KD.eq_SerialKripkeFrameClass_Logic : Logic.KD = Kripke.SerialFrameClass.logic
+  := eq_Hilbert_Logic_KripkeFrameClass_Logic
+
+
+protected abbrev KD4 : Logic := Hilbert.KD4.logic
+lemma KD4.eq_SerialTransitiveKripkeFrameClass_Logic : Logic.KD4 = Kripke.SerialTransitiveFrameClass.logic
+  := eq_Hilbert_Logic_KripkeFrameClass_Logic
+
+
+protected abbrev KD45 : Logic := Hilbert.KD45.logic
+lemma KD45.eq_SerialTransitiveEuclideanKripkeFrameClass_Logic : Logic.KD45 = Kripke.SerialTransitiveEuclideanFrameClass.logic
+  := eq_Hilbert_Logic_KripkeFrameClass_Logic
+
+
+protected abbrev KD5 : Logic := Hilbert.KD5.logic
+lemma KD5.eq_SerialEuclideanKripkeFrameClass_Logic : Logic.KD5 = Kripke.SerialEuclideanFrameClass.logic
+  := eq_Hilbert_Logic_KripkeFrameClass_Logic
+
+
+protected abbrev KDB : Logic := Hilbert.KDB.logic
+lemma KDB.eq_SerialSymmetricKripkeFrameClass_Logic : Logic.KDB = Kripke.SerialSymmetricFrameClass.logic
+  := eq_Hilbert_Logic_KripkeFrameClass_Logic
+
+
+protected abbrev KT : Logic := Hilbert.KT.logic
+lemma KT.eq_ReflexiveKripkeFrameClass_Logic : Logic.KT = Kripke.ReflexiveFrameClass.logic
+  := eq_Hilbert_Logic_KripkeFrameClass_Logic
+
+
+protected abbrev KTB : Logic := Hilbert.KTB.logic
+lemma KTB.eq_ReflexiveSymmetricKripkeFrameClass_Logic : Logic.KTB = Kripke.ReflexiveSymmetricFrameClass.logic
+  := eq_Hilbert_Logic_KripkeFrameClass_Logic
+
+
 protected abbrev S4 : Logic := Hilbert.S4.logic
-
-instance : (Logic.S4).Normal := Hilbert.normal
-
 lemma S4.eq_ReflexiveTransitiveKripkeFrameClass_Logic : Logic.S4 = Kripke.ReflexiveTransitiveFrameClass.logic
   := eq_Hilbert_Logic_KripkeFrameClass_Logic
 
 
 protected abbrev S5 : Logic := Hilbert.S5.logic
-
-instance : (Logic.S5).Normal := Hilbert.normal
-
 lemma S5.eq_ReflexiveEuclideanKripkeFrameClass_Logic : Logic.S5 = Kripke.ReflexiveEuclideanFrameClass.logic
   := eq_Hilbert_Logic_KripkeFrameClass_Logic
 
 
 protected abbrev GL : Logic := Hilbert.GL.logic
-
-instance : (Logic.GL).Normal := Hilbert.normal
-
 lemma GL.eq_TransitiveIrreflexiveFiniteKripkeFrameClass_Logic : Logic.GL = Kripke.TransitiveIrreflexiveFiniteFrameClass.logic
   := eq_Hilbert_Logic_KripkeFiniteFrameClass_Logic
 
 
 protected abbrev Grz : Logic := Hilbert.Grz.logic
-
-instance : (Logic.Grz).Normal := Hilbert.normal
-
 lemma Grz.eq_ReflexiveTransitiveAntiSymmetricFiniteKripkeFrameClass_Logic : Logic.Grz = Kripke.ReflexiveTransitiveAntiSymmetricFiniteFrameClass.logic
   := eq_Hilbert_Logic_KripkeFiniteFrameClass_Logic
 
 
 protected abbrev Triv : Logic := Hilbert.Triv.logic
-
-instance : (Logic.Triv).Normal := Hilbert.normal
-
 lemma Triv.eq_EqualityKripkeFrameClass_Logic : Logic.Triv = Kripke.EqualityFrameClass.logic
   := eq_Hilbert_Logic_KripkeFrameClass_Logic
 
 
 protected abbrev Ver : Logic := Hilbert.Ver.logic
-
 instance : (Logic.Ver).Normal := Hilbert.normal
-
 lemma Ver.eq_IsolatedFrameClass_Logic : Logic.Ver = Kripke.IsolatedFrameClass.logic
   := eq_Hilbert_Logic_KripkeFrameClass_Logic
 
@@ -106,19 +131,291 @@ open Formula
 open System
 open Kripke
 
-theorem K_ssubset_KD : Logic.K ⊂ Logic.KD := by
+theorem KTB_ssubset_S5 : Logic.KTB ⊂ Logic.S5 := by
   constructor;
-  . exact Hilbert.weakerThan_of_dominate_axioms $ by simp [axiomK!];
-  . suffices ∃ φ, Hilbert.KD ⊢! φ ∧ ¬AllFrameClass ⊧ φ by simpa [K.eq_AllKripkeFrameClass_Logic];
-    use (Axioms.D (.atom 0));
+  . rw [KTB.eq_ReflexiveSymmetricKripkeFrameClass_Logic, S5.eq_ReflexiveEuclideanKripkeFrameClass_Logic];
+    rintro φ hφ F ⟨F_refl, F_eucl⟩;
+    apply hφ;
+    refine ⟨F_refl, symm_of_refl_eucl F_refl F_eucl⟩;
+  . suffices ∃ φ, Hilbert.S5 ⊢! φ ∧ ¬ReflexiveSymmetricFrameClass ⊧ φ by simpa [KTB.eq_ReflexiveSymmetricKripkeFrameClass_Logic];
+    use Axioms.Five (.atom 0);
     constructor;
-    . exact axiomD!;
+    . exact axiomFive!;
     . apply Formula.Kripke.ValidOnFrameClass.not_of_exists_model_world;
-      let M : Model := ⟨⟨Fin 1, λ x y => False⟩, λ w _ => False⟩;
+      let M : Model := ⟨⟨Fin 3, λ x y => (x = 0) ∨ (x = 1 ∧ y ≠ 2) ∨ (x = 2 ∧ y ≠ 1)⟩, λ x _ => x = 1⟩;
+      use M, 0;
+      constructor;
+      . refine ⟨?_, ?_⟩;
+        . unfold Reflexive;
+          omega;
+        . unfold Symmetric;
+          omega;
+      . suffices (0 : M.World) ≺ 1 ∧ ∃ x : M.World, (0 : M.World) ≺ x ∧ ¬x ≺ 1 by
+          simpa [M, Semantics.Realize, Satisfies];
+        constructor;
+        . omega;
+        . use 2;
+          constructor <;> omega;
+
+theorem S4_ssubset_S5 : Logic.S4 ⊂ Logic.S5 := by
+  constructor;
+  . rw [S4.eq_ReflexiveTransitiveKripkeFrameClass_Logic, S5.eq_ReflexiveEuclideanKripkeFrameClass_Logic];
+    rintro φ hφ F ⟨F_refl, F_eucl⟩;
+    apply hφ;
+    refine ⟨F_refl, trans_of_refl_eucl F_refl F_eucl⟩;
+  . suffices ∃ φ, Hilbert.S5 ⊢! φ ∧ ¬ReflexiveTransitiveFrameClass ⊧ φ by simpa [S4.eq_ReflexiveTransitiveKripkeFrameClass_Logic];
+    use Axioms.Five (.atom 0);
+    constructor;
+    . exact axiomFive!;
+    . apply Formula.Kripke.ValidOnFrameClass.not_of_exists_model_world;
+      let M : Model := ⟨⟨Fin 3, λ x y => (x = y) ∨ (x = 0 ∧ y = 1) ∨ (x = 0 ∧ y = 2)⟩, (λ w _ => w = 2)⟩;
+      use M, 0;
+      constructor;
+      . refine ⟨?_, ?_⟩;
+        . tauto;
+        . simp [Transitive];
+          omega;
+      . suffices (0 : M.World) ≺ 2 ∧ ∃ x : M.World, (0 : M.World) ≺ x ∧ ¬x ≺ 2 by
+          simpa [M, Semantics.Realize, Satisfies];
+        constructor;
+        . tauto;
+        . use 1;
+          constructor <;> omega;
+
+theorem KD45_ssubset_S5 : Logic.KD45 ⊂ Logic.S5 := by
+  constructor;
+  . rw [KD45.eq_SerialTransitiveEuclideanKripkeFrameClass_Logic, S5.eq_ReflexiveEuclideanKripkeFrameClass_Logic];
+    rintro φ hφ F ⟨F_refl, F_eucl⟩;
+    apply hφ;
+    refine ⟨?_, ?_, F_eucl⟩;
+    . exact serial_of_refl F_refl;
+    . exact trans_of_refl_eucl F_refl F_eucl;
+  . suffices ∃ φ, Hilbert.S5 ⊢! φ ∧ ¬SerialTransitiveEuclideanFrameClass ⊧ φ by simpa [KD45.eq_SerialTransitiveEuclideanKripkeFrameClass_Logic];
+    use (Axioms.T (.atom 0));
+    constructor;
+    . exact axiomT!;
+    . apply Formula.Kripke.ValidOnFrameClass.not_of_exists_model_world;
+      let M : Model := ⟨⟨Fin 2, λ x y => (x = 0 ∧ y = 1) ∨ (x = 1 ∧ y = 1)⟩, λ x _ => x = 1⟩;
+      use M, 0;
+      constructor;
+      . refine ⟨?_, ?_, ?_⟩;
+        . intro x;
+          match x with
+          | 0 => use 1; tauto;
+          | 1 => use 1; tauto;
+        . unfold Transitive; omega;
+        . unfold Euclidean; omega;
+      . simp [Semantics.Realize, Satisfies, M];
+        tauto;
+
+theorem KB4_ssubset_S5 : Logic.KB4 ⊂ Logic.S5 := by
+  constructor;
+  . rw [KB4.eq_ReflexiveTransitiveKripkeFrameClass_Logic, S5.eq_ReflexiveEuclideanKripkeFrameClass_Logic];
+    rintro φ hφ F ⟨F_refl, F_eucl⟩;
+    apply hφ;
+    refine ⟨symm_of_refl_eucl F_refl F_eucl, trans_of_refl_eucl F_refl F_eucl⟩;
+  . suffices ∃ φ, Hilbert.S5 ⊢! φ ∧ ¬SymmetricTransitiveFrameClass ⊧ φ by simpa [KB4.eq_ReflexiveTransitiveKripkeFrameClass_Logic];
+    use (Axioms.T (.atom 0));
+    constructor;
+    . exact axiomT!;
+    . apply Formula.Kripke.ValidOnFrameClass.not_of_exists_model_world;
+      use ⟨⟨Fin 1, λ x y => False⟩, λ x _ => False⟩, 0;
+      constructor;
+      . simp [Transitive, Symmetric];
+      . simp [Semantics.Realize, Satisfies];
+
+theorem KT_ssubset_KTB : Logic.KT ⊂ Logic.KTB := by
+  constructor;
+  . exact Hilbert.weakerThan_of_dominate_axioms $ by simp;
+  . suffices ∃ φ, Hilbert.KTB ⊢! φ ∧ ¬ReflexiveFrameClass ⊧ φ by simpa [KT.eq_ReflexiveKripkeFrameClass_Logic];
+    use (Axioms.B (.atom 0));
+    constructor;
+    . exact axiomB!;
+    . apply Formula.Kripke.ValidOnFrameClass.not_of_exists_model_world;
+      let M : Model := ⟨⟨Fin 2, λ x y => x ≤ y⟩, λ w _ => w = 0⟩;
       use M, 0;
       constructor;
       . tauto;
+      . suffices ∃ x, (0 : M.World) ≺ x ∧ ¬x ≺ 0 by
+          simpa [M, Semantics.Realize, Satisfies];
+        use 1;
+        omega;
+
+theorem KDB_ssubset_KTB : Logic.KDB ⊂ Logic.KTB := by
+  constructor;
+  . rw [KDB.eq_SerialSymmetricKripkeFrameClass_Logic, KTB.eq_ReflexiveSymmetricKripkeFrameClass_Logic];
+    rintro φ hφ F ⟨F_refl, F_symm⟩;
+    apply hφ;
+    refine ⟨serial_of_refl F_refl, F_symm⟩;
+  . suffices ∃ φ, Hilbert.KTB ⊢! φ ∧ ¬SerialSymmetricFrameClass ⊧ φ by simpa [KDB.eq_SerialSymmetricKripkeFrameClass_Logic];
+    use (Axioms.T (.atom 0));
+    constructor;
+    . exact axiomT!;
+    . apply Formula.Kripke.ValidOnFrameClass.not_of_exists_model_world;
+      let M : Model := ⟨
+          ⟨Bool, λ x y => x ≠ y⟩,
+          λ x _ => x = true
+        ⟩;
+      use M, false;
+      constructor;
+      . refine ⟨?_, ?_⟩;
+        . intro x;
+          use !x;
+          simp [M];
+        . simp_all [Symmetric, M]
+      . simp [Semantics.Realize, Satisfies, M];
+        tauto;
+
+theorem KT_ssubset_S4 : Logic.KT ⊂ Logic.S4 := by
+  constructor;
+  . exact Hilbert.weakerThan_of_dominate_axioms $ by simp [axiomK!, axiomT!];
+  . suffices ∃ φ, Hilbert.S4 ⊢! φ ∧ ¬ReflexiveFrameClass ⊧ φ by simpa [KT.eq_ReflexiveKripkeFrameClass_Logic];
+    use Axioms.Four (.atom 0);
+    constructor;
+    . exact axiomFour!;
+    . apply Formula.Kripke.ValidOnFrameClass.not_of_exists_model_world;
+      let M : Model := ⟨
+          ⟨Fin 3, λ x y => (x = 0 ∧ y ≠ 2) ∨ (x = 1 ∧ y ≠ 0) ∨ (x = 2 ∧ y = 2)⟩,
+          λ w _ => w = 0 ∨ w = 1
+        ⟩;
+      use M, 0;
+      constructor;
+      . intro x; omega;
+      . suffices (∀ (y : M.World), (0 : M.World) ≺ y → y = 0 ∨ y = 1) ∧ ∃ x, (0 : M.World) ≺ x ∧ ∃ y, x ≺ y ∧ y ≠ 0 ∧ y ≠ 1 by
+          simpa [M, Semantics.Realize, Satisfies];
+        constructor;
+        . intro y hy;
+          match y with
+          | 0 => tauto;
+          | 1 => tauto;
+          | 2 => omega;
+        . use 1;
+          constructor;
+          . omega;
+          . use 2;
+            refine ⟨by omega;, by trivial, by trivial⟩;
+
+theorem KD4_ssubset_S4 : Logic.KD4 ⊂ Logic.S4 := by
+  constructor;
+  . exact Hilbert.weakerThan_of_dominate_axioms $ by simp;
+  . suffices ∃ φ, Hilbert.S4 ⊢! φ ∧ ¬SerialTransitiveFrameClass ⊧ φ by simpa [KD4.eq_SerialTransitiveKripkeFrameClass_Logic];
+    use Axioms.T (.atom 0);
+    constructor;
+    . exact axiomT!;
+    . apply Formula.Kripke.ValidOnFrameClass.not_of_exists_model_world;
+      use ⟨⟨Fin 3, λ _ y => y = 1⟩, (λ w _ => w = 1)⟩, 0;
+      constructor;
+      . refine ⟨?_, ?_⟩;
+        . simp [Serial]
+        . simp [Transitive];
       . simp [Semantics.Realize, Satisfies];
+
+theorem KD4_ssubset_KD45 : Logic.KD4 ⊂ Logic.KD45 := by
+  constructor;
+  . exact Hilbert.weakerThan_of_dominate_axioms $ by simp;
+  . suffices ∃ φ, Hilbert.KD45 ⊢! φ ∧ ¬SerialTransitiveFrameClass ⊧ φ by simpa [KD4.eq_SerialTransitiveKripkeFrameClass_Logic];
+    use Axioms.Five (.atom 0);
+    constructor;
+    . exact axiomFive!;
+    . apply Formula.Kripke.ValidOnFrameClass.not_of_exists_model_world;
+      let M : Model := ⟨
+          ⟨Fin 3, λ x y => x = y ∨ x < y⟩,
+          λ w _ => w = 0
+        ⟩;
+      use M, 0;
+      constructor;
+      . refine ⟨?_, ?_⟩;
+        . tauto;
+        . unfold Transitive;
+          omega;
+      . suffices (0 : M.World) ≺ 0 ∧ ∃ x : M.World, (0 : M.World) ≺ x ∧ ¬x ≺ 0 by
+          simpa [M, Semantics.Realize, Satisfies];
+        constructor;
+        . tauto;
+        . use 1;
+          constructor <;> omega;
+
+theorem KD5_ssubset_KD45 : Logic.KD5 ⊂ Logic.KD45 := by
+  constructor;
+  . exact Hilbert.weakerThan_of_dominate_axioms $ by simp;
+  . suffices ∃ φ, Hilbert.KD45 ⊢! φ ∧ ¬SerialEuclideanFrameClass ⊧ φ by simpa [KD5.eq_SerialEuclideanKripkeFrameClass_Logic];
+    use (Axioms.Four (.atom 0));
+    constructor;
+    . exact axiomFour!;
+    . apply Formula.Kripke.ValidOnFrameClass.not_of_exists_model_world;
+      let M : Model := ⟨⟨Fin 3, λ x y => (x = 0 ∧ y = 1) ∨ (x ≠ 0 ∧ y ≠ 0)⟩, λ w _ => w = 1⟩;
+      use M, 0;
+      constructor;
+      . refine ⟨?_, ?_⟩;
+        . intro x;
+          match x with
+          | 0 => use 1; tauto;
+          | 1 => use 1; omega;
+          | 2 => use 2; omega;
+        . unfold Euclidean; omega;
+      . suffices (∀ (y : M.World), (0 : M.World) ≺ y → y = 1) ∧ ∃ x, (0 : M.World) ≺ x ∧ ∃ y, x ≺ y ∧ y ≠ 1 by
+          simpa [M, Semantics.Realize, Satisfies];
+        constructor;
+        . intro y;
+          match y with
+          | 0 => tauto;
+          | 1 => tauto;
+          | 2 => tauto;
+        . use 1;
+          constructor;
+          . tauto;
+          . use 2;
+            constructor;
+            . omega;
+            . trivial;
+
+theorem K45_ssubset_KD45 : Logic.K45 ⊂ Logic.KD45 := by
+  constructor;
+  . exact Hilbert.weakerThan_of_dominate_axioms $ by simp;
+  . suffices ∃ φ, Hilbert.KD45 ⊢! φ ∧ ¬TransitiveEuclideanFrameClass ⊧ φ by simpa [K45.eq_TransitiveEuclideanKripkeFrameClass_Logic];
+    use Axioms.D (.atom 0);
+    constructor;
+    . exact axiomD!;
+    . apply Formula.Kripke.ValidOnFrameClass.not_of_exists_model_world;
+      let M : Model := ⟨⟨Fin 1, λ x y => False⟩, λ w _ => True⟩;
+      use M, 0;
+      constructor;
+      . simp [Transitive, Euclidean];
+      . simp [M, Semantics.Realize, Satisfies];
+
+theorem K45_ssubset_KB4 : Logic.K45 ⊂ Logic.KB4 := by
+  constructor;
+  . rw [K45.eq_TransitiveEuclideanKripkeFrameClass_Logic, KB4.eq_ReflexiveTransitiveKripkeFrameClass_Logic];
+    rintro φ hφ F ⟨F_symm, F_trans⟩;
+    apply hφ;
+    refine ⟨F_trans, eucl_of_symm_trans F_symm F_trans⟩;
+  . suffices ∃ φ, Hilbert.KB4 ⊢! φ ∧ ¬TransitiveEuclideanFrameClass ⊧ φ by simpa [K45.eq_TransitiveEuclideanKripkeFrameClass_Logic];
+    use Axioms.B (.atom 0);
+    constructor;
+    . exact axiomB!;
+    . apply Formula.Kripke.ValidOnFrameClass.not_of_exists_model_world;
+      let M : Model := ⟨⟨Fin 2, λ x y => y = 1⟩, λ w _ => w = 0⟩;
+      use M, 0;
+      constructor;
+      . refine ⟨?_, ?_⟩;
+        . tauto;
+        . unfold Euclidean; tauto;
+      . simp [M, Semantics.Realize, Satisfies];
+
+theorem KB_ssubset_KB4 : Logic.KB ⊂ Logic.KB4 := by
+  constructor;
+  . exact Hilbert.weakerThan_of_dominate_axioms $ by simp;
+  . suffices ∃ φ, Hilbert.KB4 ⊢! φ ∧ ¬SymmetricFrameClass ⊧ φ by simpa [KB.eq_SymmetricKripkeFrameClass_Logic];
+    use Axioms.Four (.atom 0);
+    constructor;
+    . exact axiomFour!;
+    . apply Formula.Kripke.ValidOnFrameClass.not_of_exists_model_world;
+      let M : Model := ⟨⟨Bool, λ x y => x != y⟩, λ w _ => w = true⟩;
+      use M, false;
+      constructor;
+      . simp [Symmetric, M];
+      . simp [M, Semantics.Realize, Satisfies];
+        tauto;
 
 theorem KD_ssubset_KT : Logic.KD ⊂ Logic.KT := by
   constructor;
@@ -133,10 +430,172 @@ theorem KD_ssubset_KT : Logic.KD ⊂ Logic.KT := by
       . tauto;
       . simp [Semantics.Realize, Satisfies];
 
-theorem K_ssubset_KT : Logic.K ⊂ Logic.KT := by
+theorem KD_ssubset_KDB : Logic.KD ⊂ Logic.KDB := by
+  constructor;
+  . exact Hilbert.weakerThan_of_dominate_axioms $ by simp;
+  . suffices ∃ φ, Hilbert.KDB ⊢! φ ∧ ¬SerialFrameClass ⊧ φ by simpa [KD.eq_SerialKripkeFrameClass_Logic];
+    use Axioms.B (.atom 0);
+    constructor;
+    . exact axiomB!;
+    . apply Formula.Kripke.ValidOnFrameClass.not_of_exists_model_world;
+      let M : Model := ⟨⟨Fin 2, λ x y => x ≤ y⟩, λ w _ => w = 0⟩;
+      use M, 0;
+      constructor;
+      . intro x;
+        match x with
+        | 0 => use 1; tauto;
+        | 1 => use 1;
+      . suffices ∃ x, (0 : M.World) ≺ x ∧ ¬x ≺ 0 by
+          simpa [M, Semantics.Realize, Satisfies];
+        use 1;
+        constructor <;> omega;
+
+theorem KB_ssubset_KDB : Logic.KB ⊂ Logic.KDB := by
+  constructor;
+  . exact Hilbert.weakerThan_of_dominate_axioms $ by simp;
+  . suffices ∃ φ, Hilbert.KDB ⊢! φ ∧ ¬SymmetricFrameClass ⊧ φ by simpa [KB.eq_SymmetricKripkeFrameClass_Logic];
+    use Axioms.D (.atom 0);
+    constructor;
+    . exact axiomD!;
+    . apply Formula.Kripke.ValidOnFrameClass.not_of_exists_model_world;
+      use ⟨⟨Fin 1, λ x y => False⟩, λ w _ => w = 0⟩, 0;
+      constructor;
+      . simp [Symmetric];
+      . simp [Semantics.Realize, Satisfies];
+
+theorem KD_ssubset_KD4 : Logic.KD ⊂ Logic.KD4 := by
+  constructor;
+  . exact Hilbert.weakerThan_of_dominate_axioms $ by simp;
+  . suffices ∃ φ, Hilbert.KD4 ⊢! φ ∧ ¬SerialFrameClass ⊧ φ by simpa [KD.eq_SerialKripkeFrameClass_Logic];
+    use Axioms.Four (.atom 0);
+    constructor;
+    . exact axiomFour!;
+    . apply Formula.Kripke.ValidOnFrameClass.not_of_exists_model_world;
+      let M : Model := ⟨⟨Bool, λ x y => x != y⟩, λ w _ => w = true⟩;
+      use M, false;
+      constructor;
+      . simp [Serial, M];
+      . simp [M, Semantics.Realize, Satisfies];
+        tauto;
+
+theorem K4_ssubset_KD4 : Logic.K4 ⊂ Logic.KD4 := by
+  constructor;
+  . exact Hilbert.weakerThan_of_dominate_axioms $ by simp;
+  . suffices ∃ φ, Hilbert.KD4 ⊢! φ ∧ ¬TransitiveFrameClass ⊧ φ by simpa [K4.eq_TransitiveKripkeFrameClass_Logic];
+    use (Axioms.D (.atom 0));
+    constructor;
+    . exact axiomD!;
+    . apply Formula.Kripke.ValidOnFrameClass.not_of_exists_model_world;
+      let M : Model := ⟨
+          ⟨Fin 1, λ x y => False⟩,
+          λ w _ => w = 0
+        ⟩;
+      use M, 0;
+      constructor;
+      . tauto;
+      . simp [M, Semantics.Realize, Satisfies];
+
+lemma K4_ssubset_S4 : Logic.K4 ⊂ Logic.S4 := by
   trans;
-  . exact K_ssubset_KD;
-  . exact KD_ssubset_KT;
+  . exact K4_ssubset_KD4
+  . exact KD4_ssubset_S4
+
+theorem KD_ssubset_KD5 : Logic.KD ⊂ Logic.KD5 := by
+  constructor;
+  . exact Hilbert.weakerThan_of_dominate_axioms $ by simp;
+  . suffices ∃ φ, Hilbert.KD5 ⊢! φ ∧ ¬SerialFrameClass ⊧ φ by simpa [KD.eq_SerialKripkeFrameClass_Logic];
+    use (Axioms.Five (.atom 0));
+    constructor;
+    . exact axiomFive!;
+    . apply Formula.Kripke.ValidOnFrameClass.not_of_exists_model_world;
+      let M : Model := ⟨⟨Fin 2, λ x y => x ≤ y⟩, λ w _ => w = 0⟩;
+      use M, 0;
+      constructor;
+      . tauto;
+      . suffices (0 : M.World) ≺ 0 ∧ ∃ x, (0 : M.World) ≺ x ∧ ¬x ≺ 0 by
+          simpa [M, Semantics.Realize, Satisfies];
+        constructor;
+        . tauto;
+        . use 1;
+          constructor <;> tauto;
+
+theorem K5_ssubset_KD5 : Logic.K5 ⊂ Logic.KD5 := by
+  constructor;
+  . exact Hilbert.weakerThan_of_dominate_axioms $ by simp;
+  . suffices ∃ φ, Hilbert.KD5 ⊢! φ ∧ ¬EuclideanFrameClass ⊧ φ by simpa [K5.eq_EuclideanKripkeFrameClass_Logic];
+    use (Axioms.D (.atom 0));
+    constructor;
+    . exact axiomD!;
+    . apply Formula.Kripke.ValidOnFrameClass.not_of_exists_model_world;
+      let M : Model := ⟨
+          ⟨Fin 1, λ x y => False⟩,
+          λ w _ => w = 0
+        ⟩;
+      use M, 0;
+      constructor;
+      . tauto;
+      . simp [M, Semantics.Realize, Satisfies];
+
+theorem K4_ssubset_K45 : Logic.K4 ⊂ Logic.K45 := by
+  constructor;
+  . exact Hilbert.weakerThan_of_dominate_axioms $ by simp;
+  . suffices ∃ φ, Hilbert.K45 ⊢! φ ∧ ¬TransitiveFrameClass ⊧ φ by simpa [K4.eq_TransitiveKripkeFrameClass_Logic];
+    use (Axioms.Five (.atom 0));
+    constructor;
+    . exact axiomFive!;
+    . apply Formula.Kripke.ValidOnFrameClass.not_of_exists_model_world;
+      let M : Model := ⟨
+          ⟨Fin 2, λ x y => x < y⟩,
+          λ w _ => w = 1
+        ⟩;
+      use M, 0;
+      constructor;
+      . simp only [Set.mem_setOf_eq, Transitive];
+        omega;
+      . suffices (0 : M.World) ≺ 1 ∧ ∃ x : M.World, (0 : M.World) ≺ x ∧ ¬x ≺ 1 by
+          simpa [M, Semantics.Realize, Satisfies];
+        constructor;
+        . trivial;
+        . use 1;
+          constructor <;> omega;
+
+theorem K5_ssubset_K45 : Logic.K5 ⊂ Logic.K45 := by
+  constructor;
+  . exact Hilbert.weakerThan_of_dominate_axioms $ by simp;
+  . suffices ∃ φ, Hilbert.K45 ⊢! φ ∧ ¬EuclideanFrameClass ⊧ φ by simpa [K5.eq_EuclideanKripkeFrameClass_Logic];
+    use (Axioms.Four (.atom 0));
+    constructor;
+    . exact axiomFour!;
+    . apply Formula.Kripke.ValidOnFrameClass.not_of_exists_model_world;
+      let M : Model := ⟨⟨Fin 3, λ x y => (x = 0 ∧ y = 1) ∨ (x ≠ 0 ∧ y ≠ 0)⟩, λ w _ => w = 1⟩;
+      use M, 0;
+      constructor;
+      . simp only [Set.mem_setOf_eq, Euclidean]; omega;
+      . suffices (∀ (y : M.World), (0 : M.World) ≺ y → y = 1) ∧ ∃ x, (0 : M.World) ≺ x ∧ ∃ z, x ≺ z ∧ ¬z = 1 by
+          simpa [M, Semantics.Realize, Satisfies];
+        constructor;
+        . intro y; tauto;
+        . use 1;
+          constructor;
+          . tauto;
+          . use 2;
+            constructor;
+            . omega;
+            . trivial;
+
+theorem K_ssubset_KD : Logic.K ⊂ Logic.KD := by
+  constructor;
+  . exact Hilbert.weakerThan_of_dominate_axioms $ by simp [axiomK!];
+  . suffices ∃ φ, Hilbert.KD ⊢! φ ∧ ¬AllFrameClass ⊧ φ by simpa [K.eq_AllKripkeFrameClass_Logic];
+    use (Axioms.D (.atom 0));
+    constructor;
+    . exact axiomD!;
+    . apply Formula.Kripke.ValidOnFrameClass.not_of_exists_model_world;
+      let M : Model := ⟨⟨Fin 1, λ x y => False⟩, λ w _ => False⟩;
+      use M, 0;
+      constructor;
+      . tauto;
+      . simp [Semantics.Realize, Satisfies];
 
 theorem K_ssubset_K4 : Logic.K ⊂ Logic.K4 := by
   constructor;
@@ -181,61 +640,26 @@ theorem K_ssubset_K5 : Logic.K ⊂ Logic.K5 := by
         use 1;
         trivial;
 
-theorem KT_ssubset_S4 : Logic.KT ⊂ Logic.S4 := by
+theorem K_ssubset_KB : Logic.K ⊂ Logic.KB := by
   constructor;
-  . exact Hilbert.weakerThan_of_dominate_axioms $ by simp [axiomK!, axiomT!];
-  . suffices ∃ φ, Hilbert.S4 ⊢! φ ∧ ¬ReflexiveFrameClass ⊧ φ by simpa [KT.eq_TransitiveKripkeFrameClass_Logic];
-    use Axioms.Four (.atom 0);
+  . exact Hilbert.weakerThan_of_dominate_axioms $ by simp [axiomK!];
+  . suffices ∃ φ, Hilbert.KB ⊢! φ ∧ ¬AllFrameClass ⊧ φ by simpa [K.eq_AllKripkeFrameClass_Logic];
+    use (Axioms.B (.atom 0));
     constructor;
-    . exact axiomFour!;
+    . exact axiomB!;
     . apply Formula.Kripke.ValidOnFrameClass.not_of_exists_model_world;
-      let M : Model := ⟨
-          ⟨
-            Fin 3,
-            λ x y =>
-              match x, y with
-              | 0, 0 => True
-              | 0, 1 => True
-              | 1, 1 => True
-              | 1, 2 => True
-              | 2, 2 => True
-              | _, _ => False
-          ⟩,
-          λ w _ => w = 0 ∨ w = 1
-        ⟩;
+      let M : Model := ⟨⟨Fin 2, λ x y => x = 0 ∧ y = 1⟩, λ w _ => w = 0⟩;
       use M, 0;
       constructor;
-      . intro x;
-        match x with
-        | 0 => tauto;
-        | 1 => tauto;
-        | 2 => tauto;
-      . suffices (∀ (y : M.World), (0 : M.World) ≺ y → y = 0 ∨ y = 1) ∧ ∃ x, (0 : M.World) ≺ x ∧ ∃ y, x ≺ y ∧ y ≠ 0 ∧ y ≠ 1 by
-          simpa [M, Semantics.Realize, Satisfies];
-        constructor;
-        . intro y hy;
-          match y with
-          | 0 => tauto;
-          | 1 => tauto;
-          | 2 => tauto;
-        . use 1;
-          constructor;
-          . tauto;
-          . use 2;
-            refine ⟨by tauto, by trivial, by trivial⟩;
+      . tauto;
+      . suffices ∃ (x : M.World), (0 : M.World) ≺ x ∧ ¬x ≺ 0 by simpa [Semantics.Realize, Satisfies, M];
+        use 1;
+        trivial;
 
-theorem K4_ssubset_S4 : Logic.K4 ⊂ Logic.S4 := by
-  constructor;
-  . apply Hilbert.K4_weakerThan_S4;
-  . suffices ∃ φ, Hilbert.S4 ⊢! φ ∧ ¬TransitiveFrameClass ⊧ φ by simpa [K4.eq_TransitiveKripkeFrameClass_Logic];
-    use Axioms.T (.atom 0);
-    constructor;
-    . exact axiomT!;
-    . apply Formula.Kripke.ValidOnFrameClass.not_of_exists_model_world;
-      use ⟨⟨Fin 3, λ _ y => y = 1⟩, (λ w _ => w = 1)⟩, 0;
-      constructor;
-      . simp [Transitive];
-      . simp [Semantics.Realize, Satisfies];
+lemma K_ssubset_KT : Logic.K ⊂ Logic.KT := by
+  trans;
+  . exact K_ssubset_KD;
+  . exact KD_ssubset_KT;
 
 theorem K4_ssubset_GL : Logic.K4 ⊂ Logic.GL := by
   constructor;
@@ -267,31 +691,6 @@ theorem S4_ssubset_Triv : Logic.S4 ⊂ Logic.Triv := by
         constructor;
         . omega;
         . trivial;
-
-theorem S4_ssubset_S5 : Logic.S4 ⊂ Logic.S5 := by
-  constructor;
-  . rw [S4.eq_ReflexiveTransitiveKripkeFrameClass_Logic, S5.eq_ReflexiveEuclideanKripkeFrameClass_Logic];
-    rintro φ hφ F ⟨F_refl, F_eucl⟩;
-    apply hφ;
-    refine ⟨F_refl, trans_of_refl_eucl F_refl F_eucl⟩;
-  . suffices ∃ φ, Hilbert.S5 ⊢! φ ∧ ¬ReflexiveTransitiveFrameClass ⊧ φ by simpa [S4.eq_ReflexiveTransitiveKripkeFrameClass_Logic];
-    use Axioms.Five (.atom 0);
-    constructor;
-    . exact axiomFive!;
-    . apply Formula.Kripke.ValidOnFrameClass.not_of_exists_model_world;
-      let M : Model := ⟨⟨Fin 3, λ x y => (x = y) ∨ (x = 0 ∧ y = 1) ∨ (x = 0 ∧ y = 2)⟩, (λ w _ => w = 2)⟩;
-      use M, 0;
-      constructor;
-      . refine ⟨?_, ?_⟩;
-        . tauto;
-        . simp [Transitive];
-          omega;
-      . suffices (0 : M.World) ≺ 2 ∧ ∃ x : M.World, (0 : M.World) ≺ x ∧ ¬x ≺ 2 by
-          simpa [M, Semantics.Realize, Satisfies];
-        constructor;
-        . tauto;
-        . use 1;
-          constructor <;> omega;
 
 end Logic
 
