Foundation/Modal/Kripke/Hilbert/KD45.lean
@@ -1,0 +1,30 @@
+import Foundation.Modal.Kripke.Hilbert.Geach
+
+namespace LO.Modal
+
+open Kripke
+open Geachean
+
+abbrev Kripke.SerialTransitiveEuclideanFrameClass : FrameClass := { F | Serial F ∧ Transitive F ∧ Euclidean F }
+
+namespace Hilbert.KD45
+
+instance Kripke.sound : Sound (Hilbert.KD45) (Kripke.SerialTransitiveEuclideanFrameClass) := by
+  convert Hilbert.Geach.Kripke.sound (G := {⟨0, 0, 1, 1⟩, ⟨0, 2, 1, 0⟩, ⟨1, 1, 0, 1⟩});
+  . exact eq_Geach;
+  . unfold SerialTransitiveEuclideanFrameClass MultiGeacheanConfluentFrameClass MultiGeachean;
+    simp [Geachean.serial_def, Geachean.euclidean_def, Geachean.transitive_def];
+
+instance Kripke.consistent : System.Consistent (Hilbert.KD45) := by
+  convert Hilbert.Geach.Kripke.Consistent (G := {⟨0, 0, 1, 1⟩, ⟨0, 2, 1, 0⟩, ⟨1, 1, 0, 1⟩});
+  exact eq_Geach;
+
+instance Kripke.complete : Complete (Hilbert.KD45) (Kripke.SerialTransitiveEuclideanFrameClass) := by
+  convert Hilbert.Geach.Kripke.Complete (G := {⟨0, 0, 1, 1⟩, ⟨0, 2, 1, 0⟩, ⟨1, 1, 0, 1⟩});
+  . exact eq_Geach;
+  . unfold SerialTransitiveEuclideanFrameClass MultiGeacheanConfluentFrameClass MultiGeachean;
+    simp [Geachean.serial_def, Geachean.euclidean_def, Geachean.transitive_def];
+
+end Hilbert.KD45
+
+end LO.Modal
